changes due to new word library but broken at this point

Syntax.v
@@ -1,7 +1,6 @@
 Require Export Bool Ascii String Fin List FunctionalExtensionality Psatz PeanoNat.
-Require Export bbv.Word Lib.VectorFacts Lib.EclecticLib.
+Require Export Lib.Word Lib.WordProperties Lib.VectorFacts Lib.EclecticLib.
 
-Export Word.Notations.
 Export ListNotations.
 
 Require Import Permutation.
@@ -10,7 +9,6 @@ Require Import ZArith.
 Global Set Implicit Arguments.
 Global Set Asymmetric Patterns.
 
-Global Open Scope word_scope.
 Global Open Scope nat_scope.
 Global Open Scope string_scope.
 Global Open Scope vector_scope.
@@ -42,7 +40,7 @@ Coercion ConstBit : word >-> ConstT.
 Fixpoint getDefaultConst (k: Kind): ConstT k :=
   match k with
     | Bool => ConstBool false
-    | Bit n => ConstBit (wzero n)
+    | Bit n => ConstBit (of_nat n 0)
     | Struct n fk fs =>
       ConstStruct fk fs (fun i => getDefaultConst (fk i))
     | Array n k => ConstArray (fun _ => getDefaultConst k)
@@ -133,7 +131,7 @@ Section Phoas.
              (i: Expr (SyntaxKind (Bit (Nat.log2_up n))))
              (v: Expr (SyntaxKind k)) :=
     BuildArray (fun i' : Fin.t n =>
-                  ITE (Eq i (Const (natToWord _ (proj1_sig (Fin.to_nat i'))))) v
+                  ITE (Eq i (Const (of_nat _ (proj1_sig (Fin.to_nat i'))))) v
                       (ReadArrayConst e i')).
 
   Definition UpdateArrayConst n k (e: Expr (SyntaxKind (Array n k)))
@@ -167,26 +165,26 @@ Section Phoas.
       UniBit (TruncMsb lsb n) (UniBit (TruncLsb (lsb + n) msb) e).
 
     Definition OneExtend msb lsb (e: Expr (SyntaxKind (Bit lsb))): Expr (SyntaxKind (Bit (lsb + msb))) :=
-      (BinBit (Concat msb lsb) (Const (wones msb))) e.
+      (BinBit (Concat msb lsb) (Const (of_nat msb ((Nat.pow 2 msb) - 1)))) e.
 
     Definition ZeroExtend msb lsb (e: Expr (SyntaxKind (Bit lsb))): Expr (SyntaxKind (Bit (lsb + msb))) :=
-      (BinBit (Concat msb lsb) (Const (wzero msb))) e.
+      (BinBit (Concat msb lsb) (Const (of_nat msb 0))) e.
 
     Definition SignExtend lsb msb: Expr (SyntaxKind (Bit lsb)) -> Expr (SyntaxKind (Bit (lsb + msb))).
       refine
         match lsb return Expr (SyntaxKind (Bit lsb)) -> Expr (SyntaxKind (Bit (lsb + msb))) with
-        | 0 => fun _ => Const (wzero msb)
+        | 0 => fun _ => Const (of_nat msb 0)
         | S m => fun e => BinBit (Concat msb (S m)) (ITE (Eq (UniBit (TruncMsb m 1)
                                                                      (castBits _ e))
-                                                             (Const (WO~0)%word))
-                                                         (Const (wzero msb))
-                                                         (Const (wones msb))) e
+                                                             (Const (of_nat 1 0)))
+                                                         (Const (of_nat msb 0))
+                                                         (Const (of_nat msb ((Nat.pow 2 msb) - 1)))) e
         end; abstract lia.
     Defined.
 
     Fixpoint replicate sz (e: Expr (SyntaxKind (Bit sz))) n : Expr (SyntaxKind (Bit (n * sz))) :=
       match n with
-      | 0 => Const WO
+      | 0 => Const (of_nat 0 0)
       | S m => BinBit (Concat (m * sz) sz) (replicate e m) e
       end.
     
@@ -238,12 +236,12 @@ Section Phoas.
     Fixpoint countLeadingZeros ni no: Expr (SyntaxKind (Bit ni)) -> Expr (SyntaxKind (Bit no)).
     refine
       match ni return Expr (SyntaxKind (Bit ni)) -> Expr (SyntaxKind (Bit no)) with
-      | 0 => fun _ => Const (wzero _)
+      | 0 => fun _ => Const ((of_nat _ 0))
       | S m => fun e =>
-                 ITE (Eq (UniBit (TruncMsb m 1) (castBits (eq_sym (Nat.add_1_r m)) e)) (Const WO~0))
-                     (CABit Add [Const (natToWord _ 1);
+                 ITE (Eq (UniBit (TruncMsb m 1) (castBits (eq_sym (Nat.add_1_r m)) e)) (Const (of_nat 1 0)))
+                     (CABit Add [Const (of_nat _ 1);
                                      countLeadingZeros m _ (UniBit (TruncLsb m 1) (castBits (eq_sym (Nat.add_1_r m)) e))])
-                     (Const (wzero _))
+                     (Const (of_nat _ 0))
       end.
     Defined.
 
@@ -273,7 +271,7 @@ Section Phoas.
           (sizes: Fin.t n -> nat)
           (f: forall i, Expr (SyntaxKind (Bit (sizes i)))),
           Expr (SyntaxKind (Bit (sumSizes sizes))) with
-      | 0 => fun _ _ => Const WO
+      | 0 => fun _ _ => Const (of_nat 0 0)
       | S m => fun sizes f =>
                  BinBit
                    (Concat _ _) (f Fin.F1)
@@ -283,7 +281,7 @@ Section Phoas.
     Fixpoint pack (k: Kind): Expr (SyntaxKind k) -> Expr (SyntaxKind (Bit (size k))).
       refine
       match k return Expr (SyntaxKind k) -> Expr (SyntaxKind (Bit (size k))) with
-      | Bool => fun e => (ITE e (Const (WO~1)%word) (Const (WO~0)%word))
+      | Bool => fun e => (ITE e (Const  (of_nat 1 ((Nat.pow 2 1) - 1))) (Const (of_nat 1 0)))
       | Bit n => fun e => e
       | Struct n fk fs =>
         fun e =>
@@ -293,11 +291,11 @@ Section Phoas.
         fun e =>
           (fix help i :=
              match i return Expr (SyntaxKind (Bit (i * size k))) with
-             | 0 => Const WO
+             | 0 => Const (of_nat 0 0)
              | S m =>
                castBits _ (BinBit
                              (Concat (size k) (m * size k))
-                             (@pack k (ReadArray e (Const (natToWord (Nat.log2_up n) m))))
+                             (@pack k (ReadArray e (Const (of_nat (Nat.log2_up n) m))))
                              (help m))
              end) n
       end; abstract lia.
@@ -332,7 +330,7 @@ Section Phoas.
 
     Fixpoint unpack (k: Kind): Expr (SyntaxKind (Bit (size k))) -> Expr (SyntaxKind k) :=
       match k return Expr (SyntaxKind (Bit (size k))) -> Expr (SyntaxKind k) with
-      | Bool => fun e => Eq e (Const (WO~1)%word)
+      | Bool => fun e => Eq e (Const  (of_nat 1 ((Nat.pow 2 1) - 1)))
       | Bit _ => fun e => e
       | Struct n fk fs =>
         fun e => BuildStruct
@@ -560,7 +558,7 @@ Definition buildNumDataArray num dataArray IdxNum Data ty (idx: ty (Bit (Nat.log
                                    ReadArray
                                      (Var ty _ val)
                                      (CABit Add (Var ty (SyntaxKind _) idx ::
-                                                     Const ty (natToWord _ (proj1_sig (Fin.to_nat i))) :: nil))))).
+                                                     Const ty (of_nat _ (proj1_sig (Fin.to_nat i))) :: nil))))).
                                                                                                                    
 Definition updateNumDataArray num dataArray IdxNum Data ty (idxData: ty (WriteRq (Nat.log2_up IdxNum)
                                                                                  (Array num Data))):
@@ -572,12 +570,12 @@ Definition updateNumDataArray num dataArray IdxNum Data ty (idxData: ty (WriteRq
                                     (UpdateArray newArr
                                                  (CABit Add (ReadStruct (Var ty (SyntaxKind _) idxData)
                                                                         Fin.F1 ::
-                                                                        Const ty (natToWord _ (proj1_sig (Fin.to_nat i))) ::
+                                                                        Const ty (of_nat _ (proj1_sig (Fin.to_nat i))) ::
                                                                         nil))
                                                  (ReadArrayConst (ReadStruct (Var ty (SyntaxKind _) idxData)
                                                                              (Fin.FS Fin.F1)) i))) (getFins num)
                                  (Var ty (SyntaxKind (Array IdxNum Data)) val))
-                      (Return (Const _ WO))).
+                      (Return (Const _ (of_nat 0 0)))).
 
 Definition updateNumDataArrayMask num dataArray IdxNum Data ty (idxData: ty (WriteRqMask
                                                                                (Nat.log2_up IdxNum) num Data)):
@@ -591,14 +589,14 @@ Definition updateNumDataArrayMask num dataArray IdxNum Data ty (idxData: ty (Wri
                                       (UpdateArray newArr
                                                    (CABit Add (ReadStruct
                                                                  (Var ty (SyntaxKind _) idxData)
-                                                                 Fin.F1 :: Const ty (natToWord _ (proj1_sig (Fin.to_nat i))) ::
+                                                                 Fin.F1 :: Const ty (of_nat _ (proj1_sig (Fin.to_nat i))) ::
                                                                  nil))
                                                    (ReadArrayConst (ReadStruct (Var ty (SyntaxKind _) idxData)
                                                                                (Fin.FS Fin.F1)) i))
                                       newArr
                                  ) (getFins num)
                                  (Var ty (SyntaxKind (Array IdxNum Data)) val))
-                      (Return (Const _ WO))).
+                      (Return (Const _ (of_nat 0 0)))).
 
 Definition readRegFile num dataArray (read: list string) IdxNum Data :=
   (map (fun x => (x, existT MethodT (Bit (Nat.log2_up IdxNum), Array num Data)
@@ -620,7 +618,7 @@ Definition readSyncRegFile (isAddr: bool) num dataArray (read: list SyncRead) Id
               existT MethodT (Bit (Nat.log2_up IdxNum), Void)
                      (fun ty idx =>
                         WriteReg (readRegName r) (Var ty (SyntaxKind _) idx)
-                                 (Return (Const _ WO)))))) read)
+                                 (Return (Const _ (of_nat 0 0))))))) read)
       ++
       (map (fun r =>
               (readResName r,
@@ -636,7 +634,7 @@ Definition readSyncRegFile (isAddr: bool) num dataArray (read: list SyncRead) Id
                      (fun ty idx =>
                         LetAction (buildNumDataArray num dataArray IdxNum Data ty idx)
                                   (fun vals => WriteReg (readRegName r) (Var ty (SyntaxKind _) vals)
-                                                        (Return (Const _ WO)))))) read)
+                                                        (Return (Const _ (of_nat 0 0))))))) read)
       ++
       (map (fun r =>
               (readResName r,
@@ -939,6 +937,7 @@ Proof.
       * right; intro; subst.
         apply (n0 eq_refl).
   - induction n.
+
     + left.
       extensionality x.
       apply Fin.case0.
@@ -967,72 +966,36 @@ Definition evalCABool (op: CABoolOp) (ws : list bool) : bool :=
     | Xor => fold_left xorb ws false
   end.
 
-Fixpoint fold_left_word (f: bool -> bool -> bool) sz (w: word sz) init: bool :=
-  match w with
-  | WO => init
-  | WS b _ rst => fold_left_word f rst (f init b)
-  end.
-
-Fixpoint fold_right_word (f: bool -> bool -> bool) init sz (w: word sz): bool :=
-  match w with
-  | WO => init
-  | WS b _ rst => f b (fold_right_word f init rst)
-  end.
-
 Definition evalUniBit n1 n2 (op: UniBitOp n1 n2): word n1 -> word n2 :=
   match op with
-  | Inv n => (@wnot n)
-  | TruncLsb lsb msb => split1 lsb msb
-  | TruncMsb lsb msb => split2 lsb msb
-  | UAnd n => fun w => WS (fold_left_word andb w true) WO
-  | UOr n => fun w => WS (fold_left_word orb w false) WO
-  | UXor n => fun w => WS (fold_left_word xorb w false) WO
+  | Inv n => (wnot n)
+  | TruncLsb lsb msb => truncLsb 
+  | TruncMsb lsb msb => truncMsb
+  | UAnd n =>  fun w => of_bool 1 (wuand n w)
+  | UOr n => fun w => of_bool 1 (wuor n w)
+  | UXor n => fun w => of_bool 1 (wuxor n w)
   end.
 
-Definition wdivN := wordBinN Nat.div.
-Definition wremN := wordBinN Nat.modulo.
-
-Definition wneg_simple sz (x: word sz) := wnot x ^+ $1.
-
-Definition wminus_simple sz (x y: word sz) := x ^+ (wneg_simple y).
-
-Lemma wneg_simple_wneg sz: forall (x: word sz), wneg_simple x = wneg x.
-Proof.
-  unfold wneg_simple.
-  intros.
-  rewrite wneg_wnot.
-  rewrite wminus_wplus_undo.
-  reflexivity.
-Qed.
-
-Lemma wminus_simple_wminus sz: forall (x y: word sz), wminus_simple x y = wminus x y.
-Proof.
-  unfold wminus_simple.
-  intros.
-  rewrite wneg_simple_wneg.
-  rewrite wminus_def.
-  reflexivity.
-Qed.
 
 Definition evalBinBit n1 n2 n3 (op: BinBitOp n1 n2 n3)
   : word n1 -> word n2 -> word n3 :=
   match op with
-    | Sub n => @wminus_simple n
-    | Div n => @wdivN n
-    | Rem n => @wremN n
-    | Sll n m => (fun x y => wlshift x (wordToNat y))
-    | Srl n m => (fun x y => wrshift x (wordToNat y))
-    | Sra n m => (fun x y => wrshifta x (wordToNat y))
-    | Concat n1 n2 => fun x y => (Word.combine y x)
+    | Sub n => wsub n
+    | Div n => wdiv n
+    | Rem n => wmod n
+    | Sll n m => fun x y => wslu _ x (of_nat _ (wordVal _ y))
+    | Srl n m =>  fun x y => wsru _ x (of_nat _ (wordVal _ y))
+    | Sra n m =>  wsra
+    | Concat n1 n2 => concat
   end.
 
 Definition evalCABit n (op: CABitOp) (ls: list (word n)): word n :=
   match op with
-    | Add => fold_left (@wplus n) ls (wzero n)
-    | Mul => fold_left (@wmult n) ls (natToWord n 1)
-    | Band => fold_left (@wand n) ls (wones n)
-    | Bor => fold_left (@wor n) ls (wzero n)
-    | Bxor => fold_left (@wxor n) ls (wzero n)
+    | Add => fold_left (wadd n) ls (of_nat n 0)
+    | Mul => fold_left (wmul n) ls (of_nat n 1)
+    | Band => fold_left (wand n) ls  (of_nat n ((Nat.pow 2 n) - 1))
+    | Bor => fold_left (wor n) ls (of_nat n 0)
+    | Bxor => fold_left (wxor n) ls (of_nat n 0)
   end.
 
 Definition evalBinBitBool n1 n2 (op: BinBitBoolOp n1 n2)
@@ -1068,7 +1031,7 @@ Definition MethsT := (list MethT).
 
 
 Section Semantics.
-  Fixpoint evalExpr exprT (e: Expr type exprT): fullType type exprT :=
+ Fixpoint evalExpr exprT (e: Expr type exprT): fullType type exprT :=
     match e in Expr _ exprT return fullType type exprT with
       | Var _ v => v
       | Const _ v => evalConstT v
@@ -1085,7 +1048,7 @@ Section Semantics.
       | ReadStruct n fk fs e i => (@evalExpr _ e) i
       | BuildStruct n fk fs fv => fun i => @evalExpr _ (fv i)
       | ReadArray n k fv i =>
-        match lt_dec (wordToNat (@evalExpr _ i)) n with
+        match lt_dec ((wordVal _ (@evalExpr _ i))) n with
         | left pf => fun fv => fv (Fin.of_nat_lt pf)
         | right _ => fun _ => evalConstT (getDefaultConst k)
         end (@evalExpr _ fv)
@@ -1324,7 +1287,7 @@ Fixpoint getNumFromCalls (f : MethT) (l : MethsT) : Z :=
   end.
 
 Definition getNumCalls (f : MethT) (l : list FullLabel) :=
-  getNumFromCalls f (concat (map (fun x => (snd (snd x))) l)).
+  getNumFromCalls f (List.concat (map (fun x => (snd (snd x))) l)).
 
 Fixpoint getNumFromExecs (f : MethT) (l : list RuleOrMeth) : Z :=
   match l with
@@ -1367,7 +1330,7 @@ Section BaseModule.
             rn rb
             (HInRules: In (rn, rb) (getRules m))
             reads u cs
-            (HAction: SemAction o (rb type) reads u cs WO)
+            (HAction: SemAction o (rb type) reads u cs (of_nat 0 0))
             (HReadsGood: SubList (getKindAttr reads)
                                  (getKindAttr (getRegisters m)))
             (HUpdGood: SubList (getKindAttr u)
@@ -1534,7 +1497,7 @@ Definition getCallsWithSignPerMeth (meth: DefMethT) :=
   getCallsWithSign (projT2 (snd meth) _ tt).
 
 Definition getCallsWithSignPerMod (m: Mod) :=
-  concat (map getCallsWithSignPerRule (getAllRules m)) ++ concat (map getCallsWithSignPerMeth (getAllMethods m)).
+  List.concat (map getCallsWithSignPerRule (getAllRules m)) ++ List.concat (map getCallsWithSignPerMeth (getAllMethods m)).
 
 Definition getCallsPerMod (m: Mod) := map fst (getCallsWithSignPerMod m).
 
@@ -1788,7 +1751,7 @@ Definition hiddenBy (meths : list DefMethT) (h : string) : bool :=
   (getBool (in_dec string_dec h (map fst meths))).
 
 Definition getAllBaseMethods (lb : list BaseModule) : (list DefMethT) :=
-  (concat (map getMethods lb)).
+  (List.concat (map getMethods lb)).
 
 Definition hiddenByBase (lb : list BaseModule) (h : string) : bool :=
   (hiddenBy (getAllBaseMethods lb) h).
