All.v
@@ -1,5 +1,4 @@
 Require Export AllNoNotations.
 (* N.b.: this module exports notations or things dependent on them *)
 Require Export KamiNotations LibStruct.
-Export Word.Notations.
 Export ListNotations.
