KamiNotations.v
@@ -54,8 +54,9 @@ Require Import RecordUpdate.RecordSet.
   (** Notations for expressions *)
 
   Notation "k @# ty" := (Expr ty (SyntaxKind k)) (no associativity, at level 98, only parsing).
-  Notation "# v" := (Var ltac:(assumption) (SyntaxKind _) v) (only parsing) : kami_expr_scope.
-  Notation "$ n" := (Const _ (natToWord _ n)): kami_expr_scope.
+
+  Notation "# v" := (Var ltac:(assumption) (SyntaxKind _) v) (at level 0, only parsing) : kami_expr_scope. 
+  Notation "$ n" := (Const _ (of_nat _ n)) (at level 9) : kami_expr_scope.
   Notation "$$ e" := (Const ltac:(assumption) e) (at level 8, only parsing) : kami_expr_scope.
 
   Notation "! v" := (UniBool Neg v) (at level 35): kami_expr_scope.
@@ -104,18 +105,18 @@ Require Import RecordUpdate.RecordSet.
   Infix ">>" := (BinBit (Srl _ _)) (at level 100) : kami_expr_scope.
   Infix ">>>" := (BinBit (Sra _ _)) (at level 100) : kami_expr_scope.
   Notation "{< a , .. , b >}" :=
-    ((BinBit (Concat _ _)) a .. (BinBit (Concat _ _) b (@Const _ (Bit 0) WO)) ..)
+    ((BinBit (Concat _ _)) a .. (BinBit (Concat _ _) b (@Const _ (Bit 0) (of_nat 0 0))) ..)
       (at level 100, a at level 99): kami_expr_scope.
   Notation "{< a , .. , b >}" :=
-    (Word.combine b .. (Word.combine a WO) ..)
+    (concat b .. (concat a (of_nat 0 0)) ..)
       (at level 100, a at level 99): word_scope.
 
   Infix "<" := (BinBitBool (LessThan _)) : kami_expr_scope.
   Notation "x > y" := (BinBitBool (LessThan _) y x) : kami_expr_scope.
   Notation "x >= y" := (UniBool Neg (BinBitBool (LessThan _) x y)) : kami_expr_scope.
   Notation "x <= y" := (UniBool Neg (BinBitBool (LessThan _) y x)) : kami_expr_scope.
-  Infix "<s" := (Slt _) : kami_expr_scope.
-  Notation "x >s y" := (Slt _ y x) : kami_expr_scope.
+  Infix "<s" := (Slt _) (at level 70) : kami_expr_scope.
+  Notation "x >s y" := (Slt _ y x) (at level 70, y at next level) : kami_expr_scope.
   Notation "x >=s y" := (UniBool Neg (Slt _ x y)) (at level 100) : kami_expr_scope.
   Notation "x <=s y" := (UniBool Neg (Slt _ y x)) (at level 100): kami_expr_scope.
   Infix "==" := Eq (at level 39, no associativity) : kami_expr_scope.
@@ -282,7 +283,7 @@ Require Import RecordUpdate.RecordSet.
   Definition writeNames (ty: Kind -> Type) k namesVals :=
     map (fun r => 
            (@WriteReg _ _ (fst r) (SyntaxKind k) (snd r)
-                      (Return (Const ty WO)))) namesVals.
+                      (Return (Const ty (of_nat 0 0))))) namesVals.
 
   (* Complex list action notations *)
   Notation "'GatherActions' actionList 'as' val ; cont" :=
@@ -314,11 +315,11 @@ Require Import RecordUpdate.RecordSet.
   Delimit Scope kami_scope with kami.
 
   Notation "'RegisterN' name : type <- init" :=
-    (MERegister (name%string, existT RegInitValT type (Some ((NativeConst init)%kami_init)%word)))
+    (MERegister (name%string, existT RegInitValT type (Some ((NativeConst init)%kami_init))))
       (at level 13, name at level 99) : kami_scope.
 
   Notation "'Register' name : type <- init" :=
-    (MERegister (name%string, existT RegInitValT (SyntaxKind type) (Some (makeConst ((init)%kami_init)%word))))
+    (MERegister (name%string, existT RegInitValT (SyntaxKind type) (Some (makeConst ((init)%kami_init)))))
       (at level 13, name at level 99) : kami_scope.
 
   Notation "'RegisterU' name : type" :=
@@ -377,11 +378,11 @@ Require Import RecordUpdate.RecordSet.
     (getStruct (cons s1%kami_struct .. (cons sN%kami_struct nil) ..)).
 
   Notation "'ARRAY_CONST' { x1 ; .. ; xn }" :=
-    (ConstArray (nth_Fin' (cons (x1%kami_init)%word .. (cons (xn%kami_init)%word nil) ..) eq_refl)).
+    (ConstArray (nth_Fin' (cons (x1%kami_init) .. (cons (xn%kami_init) nil) ..) eq_refl)).
 
   Notation "'STRUCT_CONST' { s1 ; .. ; sN }" :=
-    (getStructConst (cons (s1%struct_initial)%word ..
-                          (cons (sN%struct_initial)%word nil) ..)).
+    (getStructConst (cons (s1%struct_initial) ..
+                          (cons (sN%struct_initial) nil) ..)).
 
   Notation "i #: n" := (@Fin.of_nat_lt (i)%nat (n)%nat ltac:(lia)) (at level 10, only parsing).
 
