Lib/Word.v
@@ -1,0 +1,182 @@
+Require Import Coq.ZArith.BinIntDef Coq.ZArith.BinInt Coq.ZArith.Zdiv.
+
+
+Definition minimize_eq_proof{A: Type}(eq_dec: forall (x y: A), {x = y} + {x <> y}){x y: A}    (pf: x = y): x = y :=
+  match eq_dec x y with
+  | left p => p
+  | right n => match n pf: False with end
+  end.
+
+Section Word.
+  Section fixedWidth.
+    Variable width : nat.
+
+    Let wrap_value n := Z.modulo n (Z.pow 2 (Z.of_nat width)).
+
+    (* Word is a record with two fields wordVal and wordBound *)
+    Record word := mk {wordVal : Z ;
+                       wordBound : wrap_value wordVal = wordVal}.
+    Delimit Scope word_scope with word.
+    Bind Scope word_scope with word.
+
+    Open Scope word_scope.
+
+    Theorem Natmod_mod : forall a n, Nat.modulo (Nat.modulo a n) n = Nat.modulo a n.
+    Proof.
+      destruct n.
+      - reflexivity.
+      - rewrite Nat.mod_mod by abstract (intro; discriminate).
+        reflexivity.
+    Defined.
+    
+
+    Definition wordWrap (n : Z) : word :=
+      mk (wrap_value n) (minimize_eq_proof Z.eq_dec (Zdiv.Zmod_mod n _)).
+    
+
+    Definition ZToWord := wordWrap.
+
+    Definition boolToZ b : Z :=
+      match b with
+      | false => 0
+      | true => 1
+      end.
+
+    Definition boolToWord b := wordWrap (boolToZ b).
+
+    Definition wadd x y := wordWrap (Z.add (wordVal x) (wordVal y)).
+
+    Definition wsub x y := wordWrap (Z.sub (wordVal x) (wordVal y)).
+
+    Definition wor x y := wordWrap (Z.lor (wordVal x) (wordVal y)).
+
+    Definition wand x y := wordWrap (Z.land (wordVal x) (wordVal y)).
+
+    Definition wxor x y := wordWrap (Z.lxor (wordVal x) (wordVal y)).
+
+    Definition wnot x := wordWrap (Z.sub (Z.pow 2 (Z.of_nat width)) (Z.add (wordVal x) 1)).
+
+    Definition wuand x := Z.eqb (wordVal (wordWrap 1)) (wordVal x).
+
+    Definition wuor x := negb (Z.eqb (wordVal (wordWrap 0)) (wordVal x)).
+
+    Fixpoint pos_uxor (p : positive) : bool :=
+      match p with
+      | xH => true
+      | xI p' => negb (pos_uxor p')
+      | xO p' => (pos_uxor p')
+      end.
+
+    Definition N_uxor (n : N) : bool :=
+      match n with
+      | N0 => false
+      | Npos p => pos_uxor p
+      end.
+
+    Definition un_xor (z : Z) : bool :=
+      match z with
+      | Z0 => false
+      | Zpos p => pos_uxor p
+      | Zneg p => pos_uxor p
+      end.
+
+    Definition wuxor x := un_xor (wordVal x).
+
+    Definition wmul x y := wordWrap (Z.mul (wordVal x) (wordVal y)).
+
+    Definition wdiv x y := wordWrap (Z.div (wordVal x) (wordVal y)).
+
+    Definition wmod x y := wordWrap (Z.modulo (wordVal x) (wordVal y)).
+
+    Definition wslu x y := wordWrap (Z.mul (wordVal x) (Z.pow 2 (wordVal y))).
+
+    Definition wsru x y := wordWrap (Z.div (wordVal x) (Z.pow 2 (wordVal y))).
+
+    Definition weqb x y := Z.eqb (wordVal x) (wordVal y).
+
+    Definition wltu x y := Z.ltb (wordVal x) (wordVal y).
+
+  End fixedWidth.
+
+  Definition truncLsb {lsb outSz} (w : @word outSz) : @word lsb := 
+    ZToWord lsb (wordVal outSz w).
+
+  Definition truncMsb {msb outSz} (w : @word outSz) : @word msb :=
+    ZToWord msb (Z.div (wordVal outSz w) (Z.pow 2 (Z.of_nat (Nat.sub outSz msb)))).
+
+
+  Definition wconcat {msb lsb outSz} (w1 : @word msb) (w2 : @word lsb) :  @word outSz :=
+    ZToWord outSz (Z.add (Z.mul (wordVal msb w1) (Z.of_nat (Nat.pow 2 lsb))) (wordVal lsb w2)).
+
+  Definition get_msb {sz} (w : @word sz) : @word 1 :=
+    (@truncMsb 1 sz w).
+
+  Definition get_lsb {sz} (w : @word sz) : @word 1 :=
+    (@truncLsb 1 sz w).
+
+  Definition wordValSigned {sz} (w : @word sz) : @word sz :=
+    (ZToWord _ (Z.of_nat (Nat.pow 2 sz) - (wordVal _ w))).
+
+  Definition wsraOne {sz1 sz2} (w1 : @word sz1) (w2 : @word sz2) : @word sz1 :=
+    if (Z.ltb (wordVal _ w1) (Z.of_nat (Nat.pow 2 (sz1 - 1)))) then
+      (ZToWord _ (Z.div (wordVal _ w1) (Z.of_nat (Nat.pow 2 sz2)))) else
+      (ZToWord _ (Z.add (wordVal sz1 w1) (Z.div (wordVal _ (@wordValSigned sz1 w1)) (Z.of_nat (Nat.pow 2 sz2))))).
+
+
+  Fixpoint wsraFix {sz1 sz2 : nat} (w1 : @word sz1) (w2 : nat) : @word sz1 :=
+    match w2 with
+    | O => w1
+    | S n => @wsraOne sz1 1 (@wsraFix sz1 sz2 w1 n) (ZToWord 1 1)
+    end.
+
+  Definition wsra {sz1 sz2 : nat} (w1 : @word sz1) (w2 : @word sz2) : @word sz1 :=
+    @wsraFix _ sz2 w1 (Z.to_nat (wordVal _ w2)).
+
+  Definition whd sz (w : word (S sz)) := @truncMsb 1 _ w.
+
+  Definition wtail sz (w : word (S sz)) := @truncLsb ((S sz)-1) _ w.
+
+End Word.
+
+Module Notations.
+
+  Notation "^~" := wnot : word_scope.
+  Notation "l ^+ r" := (@wadd _ l r) (at level 50, left associativity) : word_scope.
+  Notation "l ^* r" := (@wmul _ l r) (at level 40, left associativity) : word_scope.
+  Notation "l ^- r" := (@wsub _ l r) (at level 50, left associativity) : word_scope.
+  Notation "l ^/ r" := (@wdiv _ l r) (at level 50, left associativity) : word_scope.
+  Notation "l ^% r" := (@wmod _ l r) (at level 50, left associativity) : word_scope.
+  Notation "l ^| r" := (@wor _ l r) (at level 50, left associativity) : word_scope.
+  Notation "l ^& r" := (@wand _ l r) (at level 40, left associativity) : word_scope.
+
+End Notations.
+
+(*Compute (@wadd 3 (ZToWord 3 (-2%Z)) (ZToWord 3 3)).
+
+Compute (@truncMsb 1 5 (of_nat 5 31)).
+
+Compute (@concat _ _ 4 (of_nat 2 2) (of_nat 2 3)).
+
+Compute (@of_bool 1 (@wuxor _ (of_nat 2 3))).
+
+Compute (@wsru _ (of_nat 8 167) (of_nat 8 1)).
+
+
+Compute (@wsrs _ (of_nat 8 167) (of_nat 8 1)).*)
+
+(*Compute (of_nat 2 (Nat.pow 2 2 - 2 + 1)).
+
+Compute (@get_msb _ (of_nat 3 7)).
+
+Compute (@get_lsb _ (of_nat 3 6)).
+
+Compute (@wordValSigned _ (of_nat 2 3)).
+
+Compute (@wsra 4 1 (of_nat 4 15) (of_nat 1 1)).
+
+Compute (@wsra 2 1 (of_nat 2 3) (of_nat 1 1)).
+
+Compute (@wsra 5 4 (of_nat 5 9) (of_nat 4 4)).*)
+
+
+
