Lib/WordProperties.v
@@ -1,0 +1,271 @@
+Require Import Coq.ZArith.BinIntDef Coq.ZArith.BinInt Coq.ZArith.Zdiv Eqdep.
+Require Import Lib.Word.
+Require Import Lia.
+Require Import Omega.
+
+Lemma eq_wordVal {sz} {x y : word sz} : wordVal _ x = wordVal _ y -> x = y.
+Proof.
+  intros.
+  destruct x as [x px].
+  destruct y as [y py].
+  intros.
+  simpl in *; subst; auto.
+  apply f_equal, Eqdep_dec.UIP_dec. eapply Z.eq_dec.
+Qed.
+
+
+Lemma weqb_true: forall sz (a b: word sz), weqb _ a b = true -> a = b.
+Proof.
+  intros.
+  unfold weqb in H.
+  rewrite Z.eqb_eq in H.
+  apply eq_wordVal.
+  assumption.
+Qed.
+
+
+Lemma weqb_false: forall sz (a b: word sz), weqb _ a b = false -> a <> b.
+Proof.
+  intros.
+  unfold weqb in H.
+  rewrite Z.eqb_neq in H. congruence.
+Qed.
+
+
+Definition wlt_dec : forall sz (l r : word sz), {(wltu _ l r) = true} +  {(wltu _ l r) = false}.
+Proof.
+  intros.
+  destruct (wltu sz l r).
+  left. reflexivity.
+  right.
+  reflexivity.
+Qed.
+
+Lemma weq : forall sz (x y : word sz), {x = y} + {x <> y}.
+Proof.
+  intros.
+  destruct (weqb _ x y) eqn:H.
+  apply weqb_true in H.
+  left. assumption.
+  right.
+  apply weqb_false in H.
+  assumption.
+Qed.
+
+Fixpoint nat_cast (P : nat -> Type) {n m} : n = m -> P n -> P m.
+  refine match n, m return n = m -> P n -> P m with
+         | O, O => fun _ => id
+         | S n, S m => fun pf => @nat_cast (fun n => P (S n)) n m (f_equal pred pf)
+         | _, _ => fun pf => match _ pf : False with end
+         end;
+    clear; abstract congruence.
+Defined.
+
+Lemma nat_cast_eq_rect: forall (P : nat -> Type),
+    forall (n m : nat)  (e: n = m) (pn: P n),
+      nat_cast P e pn = eq_rect n P pn m e.
+Proof.
+  destruct e.
+  revert dependent P; induction n; simpl; intros.
+  - reflexivity.
+  - rewrite IHn. reflexivity.
+Qed.
+
+Lemma nat_cast_same: forall (P: nat -> Type) (s: nat) (n: P s),
+    nat_cast P eq_refl n = n.
+Proof.
+  intros. rewrite nat_cast_eq_rect. reflexivity.
+Qed.
+
+
+Fixpoint countLeadingZerosWord ni no: word ni -> word no :=
+  match ni return word ni -> word no with
+  | 0 => fun _ => (ZToWord _ 0)
+  | S m => fun e =>
+             if (weq _ (@truncMsb 1 (m+1) (nat_cast (fun n => word n) (eq_sym (Nat.add_1_r m)) e)) (ZToWord 1 0))
+             then (wadd _ (ZToWord _ 1) (@countLeadingZerosWord m no (@truncLsb m (m+1) (nat_cast (fun n => word n) (eq_sym (Nat.add_1_r m)) e))))
+             else (ZToWord _ 0)
+  end.
+
+
+Lemma neq_wordVal sz w1 w2:
+  w1 <> w2 ->
+  wordVal sz w1 <> wordVal _ w2.
+Proof.
+  intros.
+  intro.
+  apply eq_wordVal in H0.
+  contradiction.
+Qed.
+
+Lemma boundProof sz w:
+  w mod 2^sz = w -> w < 2^sz.
+Proof.
+  intros sth0.
+  simpl.
+  pose proof (Nat.mod_upper_bound w (2 ^ sz) (@Nat.pow_nonzero 2 sz ltac:(intro; discriminate))) as sth.
+  rewrite sth0 in sth.
+  auto.
+Qed.
+
+Ltac discharge_pow_nonzero :=
+  (apply Z.pow_nonzero;
+   unfold not; intros; discriminate).
+
+Hint Rewrite
+     Z.lor_spec
+     Z.lxor_spec
+     Z.testbit_0_l
+  : Z_bitwise_no_hyps.
+
+Ltac rewrite_bitwise := repeat (autorewrite with nat_bitwise_no_hyps).
+
+Ltac bitblast := repeat f_equal; eapply Z.bits_inj_iff; unfold Nat.eqf; intros; rewrite_bitwise.
+
+Lemma boundProofZ (sz : nat) (w : Z):
+  (w mod Z.of_nat (2^sz))%Z = w -> (w < Z.of_nat (2^sz))%Z.
+Proof.
+  intros sth0.
+  assert (forall sz', 0 < Z.of_nat (2 ^ sz'))%Z. {
+    induction sz'.
+    simpl. lia.
+    simpl. 
+    lia. }
+  specialize (Z.mod_pos_bound w _ (H sz)) as TMP; destruct TMP.
+  rewrite sth0 in *; assumption.
+Qed.
+
+Lemma boundProofZ' (sz : nat) (w : Z):
+  (w mod (2^ Z.of_nat sz))%Z = w -> (w < (2^ Z.of_nat sz))%Z.
+Proof.
+  intros sth0.
+  assert (forall sz', 0 < (2 ^ Z.of_nat sz'))%Z. {
+    induction sz'.
+    simpl. lia.
+    rewrite Nat2Z.inj_succ.
+    rewrite <- Z.add_1_l.
+    rewrite Z.pow_add_r.
+    lia.
+    lia.
+    lia. }
+  specialize (Z.mod_pos_bound w _ (H sz)) as TMP; destruct TMP.
+  rewrite sth0 in *; assumption.
+Qed.
+
+Ltac arithmetizeWord :=
+  repeat match goal with
+         | w: word _ |- _ => destruct w
+         end;
+  repeat match goal with
+         | H: ?w1 <> ?w2 |- _ => match type of w1 with
+                                 | word ?sz => apply neq_wordVal in H
+                                 end; simpl in H
+         | |- ?w1 = ?w2 => match type of w1 with
+                           | word ?sz => apply eq_wordVal
+                           end; simpl
+         | H: ?w mod 2^(?sz) = ?w |- _ => pose proof (boundProofZ' sz _ H);
+                                          pose proof (inhabits H); clear H
+         end; repeat match goal with
+                     | H: inhabited ?P |- _ => destruct H
+                     end.
+
+Lemma word0_neq: forall w : word 1, w <> (ZToWord 1 0) -> w = (ZToWord 1 1).
+Proof.
+  intros.
+  arithmetizeWord.
+  assert (wordVal mod 2 ^ Z.of_nat 1 >= 0)%Z.
+  destruct wordVal.
+  lia.
+  lia.
+  apply Z.le_ge.
+  assert (0 < 2^ Z.of_nat 1)%Z as P0.
+  { lia. }
+  specialize (Z.mod_pos_bound (Z.neg p) _ P0) as TMP; destruct TMP.
+  assumption.    
+  assert (0 mod Z.pow_pos 2 1 = 0)%Z.
+  rewrite Z.pow_pos_fold in *.
+  unfold Z.modulo; auto.
+  rewrite H1 in H.
+  rewrite wordBound in H0.
+  unfold Z.modulo; simpl.
+  assert (wordVal < 2)%Z.
+  simpl in *.
+  rewrite Z.pow_pos_fold in *.
+  pose (boundProofZ' _ _ wordBound).
+  admit.
+  lia.
+  pose (boundProof _ _ wordBound).
+  lia.
+  lia.
+  omega.
+  simpl.
+  simpl.
+  simpl Z.pow_pos.
+  simpl.
+  admit.
+  omega.
+  simpl in *.
+  rewrite Z.pow_pos_fold in *.
+  
+  lia.
+Qed.
+
+Lemma wor_wzero : forall sz w, wor _ (of_nat sz 0) w = w.
+Proof.
+  intros.
+  arithmetizeWord.
+  rewrite <- H0.
+  bitblast.
+  rewrite Nat.mod_0_l by discharge_pow_nonzero.
+  rewrite Nat.testbit_0_l; simpl.
+  rewrite H0.
+  auto.
+Qed.
+
+Lemma unique_word_0 : forall a : word 0,
+    a = of_nat 0 0.
+Proof.
+  intros.
+  arithmetizeWord.
+  simpl in *.
+  auto.
+Qed.
+
+Lemma wzero_wplus: forall sz w, wadd _ (of_nat sz 0) w = w.
+Proof.
+  intros.
+  arithmetizeWord.
+  simpl in *.
+  rewrite Nat.mod_0_l by discharge_pow_nonzero.
+  simpl.
+  auto.
+Qed.
+
+Lemma wor_idemp :  forall (n : nat) (x0 : word n), wor _ x0 x0 = x0.
+Proof.
+  intros.
+  induction x0.
+  unfold wor.
+  arithmetizeWord.
+  rewrite <- H0.
+  repeat f_equal.
+  rewrite Nat.lor_diag.
+  auto.
+Qed.
+
+Lemma foo : forall (n x : nat) (w1 w2 : word n),
+    wordVal _ (@truncMsb x _ w1) < wordVal _ (@truncMsb x _ w2) -> wordVal _ w1 < wordVal _ w2.
+Proof.
+  intros.
+  arithmetizeWord.
+  admit.
+  Admitted.
+  
+
+
+
+  
+  
+
+
+  
